# (c) Epimorphics Ltd, 2012

@prefix rdf:  <http://www.w3.org/1999/02/22-rdf-syntax-ns#> .
@prefix rdfs: <http://www.w3.org/2000/01/rdf-schema#> .
@prefix owl:  <http://www.w3.org/2002/07/owl#> .
@prefix xsd:  <http://www.w3.org/2001/XMLSchema#> .
@prefix dct:  <http://purl.org/dc/terms/> .
@prefix foaf: <http://xmlns.com/foaf/0.1/> .
@prefix skos: <http://www.w3.org/2004/02/skos/core#> .
@prefix time: <http://www.w3.org/2006/time#> .

@prefix version:  <http://purl.org/linked-data/version#> .

<http://purl.org/linked-data/version>  a owl:Ontology;
    rdfs:label "Versioning ontology"@en;
    rdfs:comment "Small ontology to support versioning, irredemably OWL/full."@en;
    dct:contributor [foaf:name "Brian McBride"] ;
    dct:contributor <http://www.amberdown.net/rdf/foaf.rdf#der> ;
    dct:created "2012-10-10"^^xsd:date;
    owl:versionInfo "0.1";
    .

<http://www.amberdown.net/rdf/foaf.rdf#der> a foaf:Person;
    foaf:name "Dave Reynolds" .

version:Version a owl:Class ;
    rdfs:comment "A version of a versioned thing."@en ;
    rdfs:label "Version"@en ;
    rdfs:subClassOf owl:Thing ;
    rdfs:subClassOf [ owl:minCardinality 0; owl:onProperty dct:isReplacedBy; ] ;
    rdfs:subClassOf [ owl:cardinality    1; owl:onProperty dct:isVersionOf; ] ;
    rdfs:subClassOf [ owl:minCardinality 0; owl:onProperty dct:replaces; ] ;
    rdfs:subClassOf [ owl:cardinality    1; owl:onProperty owl:versionInfo; ] ;
  .

version:VersionedThing a owl:Class ;
    rdfs:comment "The class of things that can have multiple versions."@en ;
    rdfs:label "versioned thing"@en ;
    rdfs:subClassOf owl:Thing ;
    rdfs:subClassOf [ owl:minCardinality 0; owl:onProperty dct:hasVersion; ] ;
  .

version:currentVersion a owl:ObjectProperty;
    rdfs:comment "currentVersion relates an enduring resource to its current version"@en ;
    rdfs:domain version:VersionedThing ;
    rdfs:label "current version"@en ;
    rdfs:range version:Version ;
  .

version:interval a owl:ObjectProperty;
    rdfs:label "interval"@en ;
    rdfs:comment "interval relates a thing version to an interval during which the version was valid."@en ;
    rdfs:domain version:Version ;
    rdfs:range time:Interval ;
  .

version:rigidProperty a owl:ObjectProperty;
    rdfs:label "rigid property"@en;
    rdfs:comment "Indicates a property which does not change across versions of a VersionedThing"@en;
    rdfs:domain version:VersionedThing;
    rdfs:range  rdf:Property;
  .
